---
title: "Conceptual Exercises of Chapter 7"
output: html_notebook
---

# Question 1

## (a)
When $x \le \xi$: 
$$
a_1 = \beta_0 \\
b_1 = \beta_1 \\
c_1 = \beta_2 \\
d_1 = \beta_3
$$

## (b)
When $x \lt \xi$:
$$
a_2 = \beta_0 - \beta_4 \xi^3 \\
b_2 = \beta_1 + 3 \beta_4 \xi^2 \\
c_2 = \beta_2 - 3 \beta_4 \xi \\
d_2 = \beta_3 + \beta_4
$$

## (c)
When $x = \xi$:
$$
f_1(\xi) = \beta_0 + \beta_1 \xi + \beta_2 \xi^2 + \beta_3 \xi^3 \\
f_2(\xi)
= \beta_0 - \beta_4 \xi^3 + (\beta_1 + 3 \beta_4 \xi^2) \xi 
+ (\beta_2 - 3 \beta_4 \xi) \xi^2 + (\beta_3 + \beta_4) \xi^3
= \beta_0 + \beta_1 \xi + \beta_2 \xi^2 + \beta_3 \xi^3 \\
\therefore f_1(\xi) = f_2(\xi)
$$

## (d)
When $x = \xi$:
$$
f_1'(x) = b_1 + 2c_1x + 3d_1x^2 \\
\therefore f_1'(\xi) = \beta_1 + 2\beta_2\xi + 3\beta_3 \xi^2 \\
f_2'(x) = b_2 + 2c_2 x + 3d_2 x^2 \\
\therefore f_2'(\xi)
= \beta_1 + 3 \beta_4 \xi^2 + 2 (\beta_2 - 3 \beta_4 \xi) \xi + 3(\beta_3 + \beta_4)\xi^2
= \beta_1 + 2\beta_2\xi + 3\beta_3 \xi^2 \\
= f_1'(\xi)
$$

## (e)
When $x = \xi$:
$$
f_1''(x) = 2c_1 + 6d_1x \\
\therefore f_1''(\xi) = 2\beta_2\ + 6\beta_3 \xi \\
f_2''(x) = 2c_2 + 6d_2 x \\
\therefore f_2''(\xi)
= 2(\beta_2 - 3 \beta_4 \xi) + 6 (\beta_3 + \beta_4) \xi = 2\beta_2\ + 6\beta_3 \xi\\
= f_1''(\xi)
$$

# Question 2